it's working

extraction/chord/ml/ChordShedArrangement.ml
@@ -1,13 +1,15 @@
 open Printf
-open String
 
 open ExtractedChordShed
 
 let show_pointer p =
-  string_of_int (id_of p)
+  sprintf "(id=%d, addr=%d)" (id_of p) (addr_of p)
+
+let show_list show_item l =
+  sprintf "[%s]" (String.concat "; " (map show_item l))
 
 let show_addr_list l =
-  sprintf "[%s]" (String.concat "; " (map (sprintf "%d") l))
+  show_list string_of_int l
 
 let show_pointer_list ps =
   let strs = map show_pointer ps in
@@ -37,13 +39,34 @@ let show_timeout = function
   | KeepaliveTick -> "KeepaliveTick"
   | Request (a, p) -> sprintf "Request %d %s" a (show_payload p)
 
-(* just deliver a message *)
-let plan_deliver_only gst _ n =
-  let n' = n mod (List.length (msgs gst)) in
-  Op_deliver (n', (List.nth (msgs gst) n'))
+let picki r l =
+  let i = r (List.length l) in
+  (i, List.nth l i)
 
+let pick r l =
+  snd (picki r l)
+
+let pick_timeout gst r =
+  let hosts = filter (fun h -> List.length (timeouts gst h) > 0)
+                     (nodes gst) in
+  let h = pick r hosts in
+  let t = pick r (timeouts gst h) in
+  Op_timeout (h, t)
+
+let pick_msg gst r =
+  let (i, m) = picki r (msgs gst) in
+  Op_deliver (i, m)
+(*
+let plan_deliver_or_timeout gst _ r =
+  if List.length (msgs gst) == 0
+  then pick_timeout gst r
+  else if r 10 == 0
+  then pick_timeout gst r
+  else pick_msg gst r
+ *)
 let init_nodes =
     [10;30;50;70;90]
+
 let pred_for_init = function
   | 10 -> 90
   | 30 -> 10
@@ -65,17 +88,22 @@ let init_sigma h =
     then Some ({ ptr = mp h
               ; pred = Some (mp (pred_for_init h))
               ; succ_list = map mp (succs_for_init h)
-              ; known = mp 10
+              ; known = (mp (pred_for_init h))
               ; joined = true
               ; rectify_with = None
               ; cur_request = None
               ; delayed_queries = [] })
     else None
 
+let init_timeouts h =
+  if List.mem h init_nodes
+  then [Tick]
+  else []
+
 let init =
     { nodes = init_nodes
     ; failed_nodes = []
-    ; timeouts = (fun _ -> [])
+    ; timeouts = init_timeouts
     ; sigma = init_sigma
     ; msgs = []
     ; trace = [] }
@@ -83,13 +111,70 @@ let init =
 let implode l =
   String.init (List.length l) (List.nth l)
 
+let show_field n i (name, value) =
+  match i with
+  | 0 -> sprintf "{| %s := %s;" name value
+  | i -> if i < n
+         then sprintf "   %s := %s;" name value
+         else sprintf "   %s := %s; |}" name value
+
+let show_record l =
+  String.concat "\n" (List.mapi (show_field (List.length l)) l)
+
+let show_st_cur_request st = "TODO show_st_cur_request"
+
+let show_state st =
+  show_record [ ("pred", show_opt_pointer st.pred)
+              ; ("succ_list", show_pointer_list st.succ_list)
+              ; ("known", show_pointer st.known)
+              ; ("joined", string_of_bool st.joined)
+              ; ("rectify_with", show_opt_pointer st.rectify_with)
+              ; ("cur_request", show_st_cur_request st)]
+
+let show_state_for n h =
+  match n.sigma h with
+  | None -> "NO STATE FOUND"
+  | Some st -> show_state st
+
+let info_header_for dead =
+  if dead
+  then sprintf "NODE %d (dead)"
+  else sprintf "NODE %d"
+
+let show_node_info n h =
+  let dead = List.mem h n.failed_nodes in
+  let header = info_header_for dead h in
+  String.concat "\n"
+                [ "STATE AT " ^ header
+                ; show_state_for n h
+                ; "TIMEOUTS AT " ^ header
+                ; show_list show_timeout (timeouts n h) ]
+
+let show_msg (src, (dst, p)) = 
+  sprintf "%d -> %d: %s" src dst (show_payload p)
+
+let show_net n =
+  let node_strs = "NODES" :: map (show_node_info n) (nodes n) in
+  let msgs_strs = ["MESSAGES"; show_list show_msg (msgs n)] in
+  String.concat "\n" (node_strs @ msgs_strs)
+
+let show_operation = function
+  | Op_start (a, ks) -> 
+      sprintf "op_start %d %s" a (show_addr_list ks)
+  | Op_fail a -> 
+      sprintf "op_fail %d" a
+  | Op_timeout (a, t) ->
+      sprintf "op_timeout %d %s" a (show_timeout t)
+  | Op_deliver (n, (src, (dst, p))) ->
+      sprintf "op_deliver %d %d %d %s" n src dst (show_payload p)
+
 module ChordArrangement = struct
   type net = chord_net
   type operation = chord_operation
   type netpred = chord_netpred
   type tracepred = chord_tracepred
-  let show_net n = ""
-  let show_operation o = ""
+  let show_net = show_net
+  let show_operation = show_operation
   let inits =
     [("hardcoded", init)]
   let np_name np = implode np.np_name
@@ -99,14 +184,13 @@ module ChordArrangement = struct
   let tracepreds =
     [const_true_tracepred]
   let plans =
-    [("deliver_only", plan_deliver_only)]
+    [("deliver_or_timeout", chord_plan_deliver_or_timeout)]
   type test_state = chord_test_state
-  let ts_latest ts = (ts.ts_latest)
-  let ts_trace ts = (ts.ts_trace)
-  let ts_netpreds ts = (ts.ts_netpreds)
-  let ts_tracepreds ts = (ts.ts_tracepreds)
+  let ts_latest ts = ts.ts_latest
+  let ts_trace ts = ts.ts_trace
+  let ts_netpreds ts = ts.ts_netpreds
+  let ts_tracepreds ts = ts.ts_tracepreds
   let mk_init_state = chord_mk_init_state
-  let show_state ts = ""
   let advance_test ts op = chord_advance_test ts op
 end
 (*
