extraction/lib/ShedShim.ml
@@ -1,5 +1,6 @@
 open List
-open Random
+open Printf
+
 
 module type SHED_ARRANGEMENT = sig
     type net
@@ -16,16 +17,15 @@ module type SHED_ARRANGEMENT = sig
     val tracepreds : tracepred list
     (* assoc list from names to fns for operation generation (first
        integer is the number of steps taken so far, second is a
-       randomly generated integer in the range 0 to 2^16). *)
-    val plans : (string * (net -> int -> int -> operation)) list
+       randomly generated integer in the range 0 to 2^16 - 1). *)
+    val plans : (string * (net -> int -> (int -> int) -> operation option)) list
     type test_state
     val ts_latest : test_state -> net
     val ts_trace : test_state -> (net * operation) list
     val ts_netpreds : test_state -> (netpred * bool list) list
     val ts_tracepreds : test_state -> (tracepred * (bool option) list) list
     val mk_init_state : net -> netpred list -> tracepred list -> test_state
-    val show_state : test_state -> string
-    val advance_test : test_state -> operation -> test_state
+    val advance_test : test_state -> operation -> test_state option
 end
 
 let explode s =
@@ -39,12 +39,13 @@ module Shim (A: SHED_ARRANGEMENT) = struct
     type cfg =
         { netpreds : A.netpred list
         ; tracepreds : A.tracepred list
-        ; plan : A.net -> int -> int -> A.operation
+        ; plan : A.net -> int -> (int -> int) -> A.operation option
         ; init : A.net
         ; depth : int }
 
     let print_occ occ =
-      print_endline (A.show_operation (snd occ))
+      print_endline (A.show_operation (snd occ));
+      print_endline (A.show_net (fst occ))
 
     let print_np_res i (np, l) = 
       print_endline (A.np_name np ^ ": " ^ string_of_bool (nth l i))
@@ -58,13 +59,16 @@ module Shim (A: SHED_ARRANGEMENT) = struct
       print_endline (A.tp_name tp ^ ": " ^ show_tp_result (nth l i))
 
     let print_step res i occ =
+      printf "STEP %d\n" (i + 1);
       print_occ occ;
       iter (print_np_res i) (A.ts_netpreds res);
-      iter (print_tp_res i) (A.ts_tracepreds res)
+      iter (print_tp_res i) (A.ts_tracepreds res);
+      print_newline ()
 
     let print_res res =
       iteri (print_step res) (A.ts_trace res);
       print_endline "";
+      print_endline "FINAL STATE";
       print_endline (A.show_net (A.ts_latest res))
 
     let find_np_by_name s =
@@ -76,23 +80,46 @@ module Shim (A: SHED_ARRANGEMENT) = struct
     let combine_with_nils l =
       combine l (map (fun _ -> []) l)
 
+    type test_result =
+      | Ok of A.test_state
+      | Stalled of A.test_state
+      | Failed of A.test_state * A.operation
+
+    let random_nat n =
+      if n == 0
+      then 0
+      else Random.int n
+
     let rec test_loop st plan n =
       if n <= 0
-      then st
+      then Ok st
       else
-        let rand = 5 in
-        let st' = A.advance_test st (plan (A.ts_latest st) n rand)  in
-           test_loop st' plan (n - 1)
+        match plan (A.ts_latest st) n random_nat with
+        | None -> Stalled st
+        | Some op ->
+           match A.advance_test st op with
+           | None -> Failed (st, op)
+           | Some st' -> test_loop st' plan (n - 1)
 
     let run_test cfg =
       let st = A.mk_init_state cfg.init cfg.netpreds cfg.tracepreds in
-      let res = test_loop st cfg.plan cfg.depth in
-      print_res res
+      match test_loop st cfg.plan cfg.depth with
+      | Ok res -> print_res res
+      | Failed (res, op) ->
+         print_endline "!!! invalid operation !!!";
+         print_endline (A.show_operation op);
+         print_newline ();
+         print_res res
+      | Stalled res ->
+         print_endline "!!! couldn't plan anything !!!";
+         print_newline ();
+         print_res res
 
     let main = 
+      Random.self_init ();
       let nps = ref [] in
       let tps = ref [] in
-      let n = ref 5 in
+      let n = ref 50 in
       let init = ref (fst (hd A.inits)) in
       let plan = ref (fst (hd A.plans))  in
       let add_np s = nps := find_np_by_name s :: !nps in
@@ -104,6 +131,7 @@ module Shim (A: SHED_ARRANGEMENT) = struct
           ; ("-depth", Arg.Set_int n, "number of steps to take")
           ; ("-init", Arg.Set_string init, "name of initial state") ] in
       Arg.parse opts (fun _ -> ()) "todo";
+      Printf.printf "running plan %s\n" !plan;
       run_test { netpreds = !nps
                ; tracepreds = !tps
                ; init = assoc !init A.inits 
