extraction/chord/coq/ExtractChord.v
@@ -23,25 +23,17 @@ Definition handleTick : addr -> data -> res :=
 Definition handleTimeout : addr -> data -> timeout -> res :=
   timeout_handler hash.
 
-Definition chord_net : Set :=
-  net.
-
-Definition chord_operation : Type :=
-  operation.
-
-Definition chord_run : chord_net -> chord_operation -> option chord_net :=
-  run SUCC_LIST_LEN hash.
-
-Definition chord_test_state :=
-  test_state SUCC_LIST_LEN hash.
-
-Definition chord_advance_test : chord_test_state -> chord_operation -> chord_test_state :=
-  advance_test SUCC_LIST_LEN hash.
-
+Definition chord_net := net.
+Definition chord_operation := operation.
+Definition chord_run := run SUCC_LIST_LEN hash.
+Definition chord_test_state := test_state SUCC_LIST_LEN hash.
+Definition chord_advance_test := advance_test SUCC_LIST_LEN hash.
 Definition chord_netpred := netpred.
 Definition chord_tracepred := tracepred SUCC_LIST_LEN hash.
 Definition chord_mk_init_state := mk_init_state SUCC_LIST_LEN hash.
 Definition const_true_tracepred := tp_const_true SUCC_LIST_LEN hash.
+Definition chord_plan_deliver_or_timeout := plan_deliver_or_timeout SUCC_LIST_LEN hash.
+
 Extraction "extraction/chord/coq/ExtractedChord.ml" init handleNet handleTick handleTimeout is_request closes_request.
 
-Extraction "extraction/chord/coq/ExtractedChordShed.ml" chord_net chord_operation chord_netpred chord_tracepred all_nodes_live_netpred const_true_tracepred chord_test_state chord_advance_test chord_mk_init_state.
+Extraction "extraction/chord/coq/ExtractedChordShed.ml" chord_net chord_operation chord_netpred chord_tracepred all_nodes_live_netpred const_true_tracepred chord_test_state chord_advance_test chord_mk_init_state chord_plan_deliver_or_timeout.
